transformations/Moore2Mealy/MealyWF.v
@@ -40,7 +40,45 @@ Proof.
   }
 Qed.
 
-Lemma in_find : (* fixme : use the concept of discriminant proposition for the proof *)
+Lemma In_transition : forall (m:Mealy.M) e,
+         List.In (TransitionElement e) (Model.modelElements m) <-> List.In e
+    (OptionListUtils.lift_list (get_E_data Transition_K)
+       (Model.modelElements m)).
+Proof.
+  intros m e.
+  split ; intro H.
+  {
+    apply OptionListUtils.In_lift.
+    exists (TransitionElement e). auto.
+  }  
+  {
+    apply OptionListUtils.In_lift in H.
+    destruct H as (e2 & (G & IN2)).
+    destruct e2 ; [ discriminate G | PropUtils.inj G]. 
+    assumption.
+  }
+Qed.
+
+
+Lemma discr  (m : M) : 
+  unique_ids m ->
+  forall (i : NodeId),
+    ListUtils.discriminating_predicate
+      (fun x : State_t => NodeId_beq i (State_id x) = true)
+      (OptionListUtils.lift_list (get_E_data State_K)
+         (Model.modelElements m)).
+Proof.
+  intros WF i.
+  unfold ListUtils.discriminating_predicate ; intros.
+  apply WF.
+  apply In_state ; assumption.
+  apply In_state ; assumption.
+  apply internal_NodeId_dec_bl in H1, H2.
+  congruence.
+Qed.
+
+
+Lemma in_find : 
   forall m n e,
     unique_ids m ->
     List.In (StateElement e) m.(Model.modelElements) ->
@@ -52,19 +90,10 @@ Lemma in_find : (* fixme : use the concept of discriminant proposition for the p
          Some e.
 Proof.
   intros.
-  rewrite OptionListUtils.find_lift_filter_lift.
-  destruct e ; simpl in * ; subst.
-  match goal with [ |- ?F = _] => destruct F eqn:E ; [ | exfalso ] end.
-  + f_equal. 
-    apply List.find_some in E.
-    destruct E as (IN2 & EQ).
-    apply In_state in IN2.
-    apply internal_NodeId_dec_bl in EQ. subst. apply H ; auto.
-  + apply List.find_none with (x:= {| State_id := n |}) in E ; [ |  ].
-    unfold State_id in E.
-     rewrite internal_NodeId_dec_lb in E. discriminate.
-     reflexivity.
-     apply In_state.  assumption.
+  eapply OptionListUtils.in_find_lift ; [ | | | exact H0 ].
+  { apply discr. assumption. }
+  { reflexivity. }
+  { apply internal_NodeId_dec_lb. auto. }  
 Qed.
 
 
@@ -75,3 +104,4 @@ Definition determinist m :=
       List.In t2 (State_outTransitions m s) ->
       t1.(Transition_input) = t2.(Transition_input) ->
       t1 = t2.
+
