transformations/Moore2Mealy/theorems/Elements.v
@@ -9,14 +9,43 @@ Import OptionUtils.
 Definition convert (s:Moore.State_t) : Mealy.State_t :=
   {| Mealy.State_id := s.(Moore.State_id) |}.
 
+Lemma convert_injective : 
+  forall m s1 s2,
+    MooreWF.unique_ids m ->
+    List.In (Moore.StateElement s1) m.(Model.modelElements) ->
+    List.In (Moore.StateElement s2) m.(Model.modelElements) ->
+    convert s1 = convert s2 ->
+    s1 = s2.
+Proof.
+  intros m s1 s2 WF H1 H2 H3.
+  apply WF ; auto.
+  destruct s1, s2 ; unfold convert in H3 ; congruence.
+Qed.
+
+
 Definition convert_transition  (m: Moore.M)  (t : Moore.Transition_t)   :option Mealy.Transition_t :=
   match Moore.getTransition_target m t with
   | None => None
   | Some s => Some (Mealy.Build_Transition_t t.(Moore.Transition_id) t.(Moore.Transition_input) s.(Moore.State_output))
   end.
 
+
+Lemma convert_transition_injective : 
+  forall m t1 t2 a, 
+    convert_transition m t1 = Some a -> (* would be false with None *)
+    convert_transition m t2 = Some a ->
+    t1 = t2.
+Proof.
+  unfold convert_transition ; intros.
+  PropUtils.destruct_match H ; [ PropUtils.inj H | discriminate H].
+  PropUtils.destruct_match H0 ; [ PropUtils.inj H0 | discriminate H0].
+  
+  destruct t1, t2 ; simpl in * ; congruence.
+Qed.
+
+
 Lemma convert_transition_ok : forall (m:Moore.M) t,
-    Moore.WF1 m ->
+    Moore.WF_target m ->
     List.In (Moore.TransitionElement t) m.(Model.modelElements) -> 
     SUCCESS (convert_transition m t).
 Proof.
@@ -31,8 +60,10 @@ Proof.
   + PropUtils.inj H.
     reflexivity.
   + discriminate.
-Qed.  
+Qed.
 
+Notation transform_element_fw := 
+  (Tactics.transform_element_fw  (tc := Moore2Mealy.Moore2MealyTransformationConfiguration)).
 
 Lemma state_element_fw : 
   forall (s:Moore.State_t) (m:Moore.M),
@@ -40,18 +71,8 @@ Lemma state_element_fw :
     List.In (Mealy.StateElement (convert s))  (Semantics.execute  Moore2Mealy.Moore2Mealy m).(Model.modelElements).
 Proof.
   intros s m IN.
-  eapply Tactics.in_modelElements_execute_left.
-  + apply Certification.allTuples_incl_length.
-    apply ListUtils.incl_singleton.
-    exact IN.
-    compute ; auto.
-  + apply List.in_eq. (* first rule *)
-  + reflexivity.
-  + compute. left. reflexivity.
-  + apply List.in_eq. 
-  + destruct s.
-    simpl.
-    reflexivity.
+  eapply transform_element_fw ; eauto. 
+  compute ; auto.
 Qed.
 
 Lemma state_element_bw :
